Core/LogicPaco.v
@@ -12,7 +12,7 @@ From LHL.Util Require Import
 
 From Paco Require Import paco.
 
-Inductive paco_safeF {E F A} {VE : Spec E} {VF : Spec F} i (R G : Relt VE VF) (Q : Post VE VF A) (rec : Relt VE VF -> Prog E A -> Prop) : Relt VE VF -> Prog E A -> Prop :=
+Inductive paco_safeF {T E F A} {VE : Spec T E} {VF : Spec T F} i (R G : Relt VE VF) (Q : Post VE VF A) (rec : Relt VE VF -> Prog E A -> Prop) : Relt VE VF -> Prog E A -> Prop :=
 | SafeReturn v P :
     P ==> Q v ->
     paco_safeF i R G Q rec P (Return v)
@@ -31,9 +31,9 @@ Inductive paco_safeF {E F A} {VE : Spec E} {VF : Spec F} i (R G : Relt VE VF) (Q
     paco_safeF i R G Q rec P (NoOp C)
 .
 
-Definition paco_safe {E F A} {VE : Spec E} {VF : Spec F} i (R G P : Relt VE VF) (C : Prog E A) (Q : Post VE VF A) : Prop := paco2 (paco_safeF i R G Q) bot2 P C.
+Definition paco_safe {T E F A} {VE : Spec T E} {VF : Spec T F} i (R G P : Relt VE VF) (C : Prog E A) (Q : Post VE VF A) : Prop := paco2 (paco_safeF i R G Q) bot2 P C.
 
-Lemma safe_monotone {E F A} {VE : Spec E} {VF : Spec F} (i : ThreadName) (R G : Relt VE VF) (Q : Post VE VF A) :
+Lemma safe_monotone {T E F A} {VE : Spec T E} {VF : Spec T F} (i : Name T) (R G : Relt VE VF) (Q : Post VE VF A) :
   monotone2 (paco_safeF i R G Q).
 unfold monotone2. intros.
 destruct IN.
@@ -47,7 +47,7 @@ apply LE. easy.
 Qed.
 Hint Resolve safe_monotone : paco.
 
-CoFixpoint paco_eqv_help {E F A} {VE : Spec E} {VF : Spec F} (i : ThreadName) (R G : Relt VE VF) (Q : Post VE VF A) (P : Relt VE VF) (C : Prog E A):
+CoFixpoint paco_eqv_help {T E F A} {VE : Spec T E} {VF : Spec T F} (i : Name T) (R G : Relt VE VF) (Q : Post VE VF A) (P : Relt VE VF) (C : Prog E A):
   paco_safe i R G P C Q -> SafeProg i R G P C Q.
 intros.
 punfold H.
@@ -65,7 +65,7 @@ apply paco_eqv_help. easy.
 destruct H1.
 Qed.
 
-Lemma paco_eqv {E F A} {VE : Spec E} {VF : Spec F} (i : ThreadName) (R G : Relt VE VF) (Q : Post VE VF A) (P : Relt VE VF) (C : Prog E A):
+Lemma paco_eqv {T E F A} {VE : Spec T E} {VF : Spec T F} (i : Name T) (R G : Relt VE VF) (Q : Post VE VF A) (P : Relt VE VF) (C : Prog E A):
   SafeProg i R G P C Q = paco_safe i R G P C Q.
 apply propositional_extensionality.
 split; intros.
