Examples/Snapshot.v
@@ -9,63 +9,90 @@ From LHL.Core Require Import
   Linearizability.
 
 From LHL.Examples Require Import
-  CellSpec
+  MRSWCellSpec
+  LocalVarSpec
   ThreadLocal
-  WriteSnapshotSpec.
+  NameSpec
+  SnapshotSpec.
 
 From LHL.Util Require Import
   Tactics
   TransUtil
   Util.
 
-From Coq Require Import
-  Strings.String.
+Definition E T A :=
+  LocalSig (CellSig A) |+|
+  LocalSig (VarSig (set A * set A)) |+|
+  LocalSig (VarSig nat) |+|
+  NameSig T.
 
-Definition Underlay A :=
-  LocalSig (CellSig A) |+| LocalSig (CellSig (set A * set A)) |+| LocalSig (CellSig nat).
-Definition VE A : Spec (Underlay A) :=
-  tensorSpec (localSpec (cellSpec _))(tensorSpec (localSpec (cellSpec _)) (localSpec (cellSpec _))).
+Definition VE T A : Spec T (E T A) :=
+  tensorSpec
+    (localSpec cellSpec)
+    (tensorSpec
+      (localSpec varSpec)
+      (tensorSpec
+        (localSpec varSpec)
+        nameSpec)).
+
+Definition F A := SnapshotSig A.
+Definition VF T A := @snapshotSpec T A.
 
 Definition bool_prop (P : Prop) : bool :=
   if classicT P then true else false.
 
+Definition cellsState {T A} (s : InterState (F A) (VE T A)) : Name T -> State cellSpec :=
+  LState (snd s).
+
+Definition setsState {T A} (s : InterState (F A) (VE T A)) : Name T -> State varSpec :=
+  LState (RState (snd s)).
+
+Definition ixState {T A} (s : InterState (F A) (VE T A)) : Name T -> State varSpec :=
+  LState (RState (RState (snd s))).
+
+Definition nameState {T A} (s : InterState (F A) (VE T A)) : State nameSpec :=
+  RState (RState (RState (snd s))).
+
 (* fst is old, snd is new *)
-Definition query {n} {A} self : Prog (Underlay A) (set A) :=
-  call (At self (Write (emp, emp)));;
+Definition update {T A} (v : A) : Prog (E T A) (set A) :=
+  self <- call Self;
+  let self := proj1_sig self in
+  call (At self (Write v));;
+  call (At self (Put (emp, insert v emp)));;
   while (
-    sets <- call (At self Read);
-    ret (fst sets /=? snd sets)
+    old_new <- call (At self Get);
+    ret (bool_prop (fst old_new <> snd old_new))
   ) (
-    call (At self (Write 0));;
-    (* get old *)
+    call (At self (Put 0));;
+    old_new <- call (At self Get);
+    call (At self (Put (snd old_new, emp)));;
     while (
-      i <- call (At self Read);
-      ret (bool_prop (i < n))
+      i <- call (At self Get);
+      ret (bool_prop (i < T))
     ) (
-      i <- call (At self Read);
+      i <- call (At self Get);
       v <- call (At i Read);
-      sets <- call (At self Read);
-      call (At self (Write (insert (fst sets) v, snd sets)))
-    );;
-    call (At self (Write 0));;
-    (* get new *)
-    while (
-      i <- call (At self Read);
-      ret (bool_prop (i < n))
-    ) (
-      i <- call (At self Read);
-      v <- call (At i Read);
-      sets <- call (At self Read);
-      call (At self (Write (fst sets, insert (snd sets) v)))
+      old_new <- call (At self Get);
+      call (At self (Put (fst old_new, insert v (snd old_new))));;
+      call (At self (Put (i + 1)))
     )
   );;
-  sets <- call (At self Read);
-  ret (fst sets).
+  old_new <- call (At self Get);
+  ret (snd old_new).
 
-Definition update {A} self (v : A) : Prog (Underlay A) unit :=
-  call (At self (Write v)).
-
-(* Definition snapshotImpl n A : Impl (Underlay A) (SnapshotSig A) :=
+Definition snapshotImpl T A : Impl (E T A) (SnapshotSig A) :=
   fun i m => match m with
   | Update v => update v
-  end. *)
+  end.
+
+Definition Relt T A := Relt (VE T A) (VF T A).
+Definition Prec T A := Prec (VE T A) (VF T A).
+Definition Post T A := Post (VE T A) (VF T A).
+
+Definition Inv {T A}
+  (sm : VarPend T (set A * set A))
+  (am : VarPend T nat)
+  (cm : CellPend T A)
+  : Name T -> Prec T A :=
+  fun i s ρs =>
+    True.
