Examples/CASSpec.v
@@ -1,0 +1,60 @@
+From LHL.Core Require Import
+  Program
+  Specs.
+
+From LHL.Util Require Import
+  Util.
+
+Variant CASSig {A} : ESig :=
+| CAS (v : option A) (v' : option A) : CASSig bool
+| Get : CASSig (option A).
+Arguments CASSig : clear implicits.
+
+Record CASPend {T A} := MkCASPend {
+  CASThread : Name T;
+  CASRetTy : Type;
+  CASName : CASSig A CASRetTy
+}.
+Arguments CASPend : clear implicits.
+Arguments MkCASPend {T A} _ {_}.
+
+Variant CASState {T A} :=
+| CASDef (v : option A) (m : option (CASPend T A)). (* currently value and pending call *)
+Arguments CASState : clear implicits.
+
+Variant CASStep {T A} : CASState T A -> ThreadEvent T (CASSig A) -> CASState T A -> Prop :=
+| CASCallCAS i a e n :
+    CASStep
+      (CASDef a None)
+      (i, CallEv (CAS e n))
+      (CASDef a (Some (MkCASPend i (CAS e n))))
+| CASSucc i a e n :
+    a = e ->
+    CASStep
+      (CASDef a (Some (MkCASPend i (CAS e n))))
+      (i, RetEv (CAS e n) true)
+      (CASDef n None)
+| CASFail i a e n :
+    a <> e ->
+    CASStep
+      (CASDef a (Some (MkCASPend i (CAS e n))))
+      (i, RetEv (CAS e n) false)
+      (CASDef a None)
+| CASCallGet i a :
+    CASStep
+      (CASDef a None)
+      (i, CallEv Get)
+      (CASDef a (Some (MkCASPend i Get)))
+| CASRetGet i a :
+    CASStep
+      (CASDef a (Some (MkCASPend i Get)))
+      (i, RetEv Get a)
+      (CASDef a None).
+
+Program Definition casSpec {T A} : Spec T (CASSig A) := {|
+  State := CASState T A;
+  Step := CASStep;
+  Init := CASDef None None
+|}.
+
+Admit Obligations.
