Examples/Exchanger.v
@@ -1,0 +1,552 @@
+From LHL.Core Require Import
+  ProgramRules
+  LogicFacts
+  Program
+  Traces
+  Tensor
+  Logic
+  Specs.
+
+From LHL.Util Require Import
+  Tactics
+  Util.
+
+From LHL.Examples Require Import
+  ExchangerSpec
+  ThreadLocal
+  CASSpec.
+
+From Coq Require Import
+  Logic.FunctionalExtensionality
+  Logic.PropExtensionality
+  Program.Equality.
+
+From Paco Require Import
+  paco.
+
+(* Signature *)
+
+Variant Flag := Offered | Accepted.
+
+Definition Offer A : Type := Flag * A.
+
+Notation OFFERED v := (Some (Offered, v)).
+Notation ACCEPTED v := (Some (Accepted, v)).
+
+Definition E A :=
+  CASSig (Offer A).
+
+Definition VE T A : Spec T (E A) :=
+  casSpec.
+
+Definition F A := ExchSig A.
+
+Definition VF T A : Spec T (F A) :=
+  exchSpec.
+
+(* Code *)
+
+Definition exch {A} (v : A) : Prog (E A) (option A) :=
+  my_offer_placed <- call (CAS None (OFFERED v));
+  if my_offer_placed : bool then
+    no_change <- call (CAS (OFFERED v) None);
+    if no_change : bool then
+      ret None
+    else
+      w <- call Get;
+      match w : option (Offer A) with
+      | Some (_, w) =>
+          call (CAS (ACCEPTED w) None);;
+          ret (Some w)
+      | None =>
+          ret None (* impossible *)
+      end
+  else
+    w <- call Get;
+    match w : option (Offer A) with
+    | Some (_, w) =>
+        my_offer_accepted <- call (CAS (OFFERED w) (ACCEPTED v));
+        if my_offer_accepted : bool then
+          ret (Some w)
+        else
+          ret None
+    | None =>
+        ret None
+    end.
+
+Definition exchImpl A : Impl (E A) (F A) :=
+  fun i m => match m with
+  | Exch v => exch v
+  end.
+
+(* Conditions *)
+
+Definition Relt T A := Relt (VE T A) (VF T A).
+Definition Prec T A := Prec (VE T A) (VF T A).
+Definition Post T A := Post (VE T A) (VF T A).
+
+Definition SPrec T A :=
+  InterState (F A) (VE T A) -> Poss (VF T A) -> Prop.
+
+Definition SPrecToPrec {T A} (P : SPrec T A) : Prec T A :=
+  fun s ρs => exists ρ, ρs = eq ρ /\ P s ρ.
+
+Definition CCleared {A T} : SPrec T A :=
+  fun s ρ =>
+    snd s = CASDef None None /\
+    PState ρ = ExchDef {} {}.
+
+Definition COffered {A T} (i : Name T) (v : A) : SPrec T A :=
+  fun s ρ =>
+    snd s = CASDef (OFFERED v) None /\
+    PState ρ = ExchDef {i => v} {}.
+
+Definition CAccepted {A T} (i j : Name T) (v w : A) : SPrec T A :=
+  fun s ρ =>
+    i <> j /\
+    snd s = CASDef (ACCEPTED v) None /\
+    PState ρ = ExchDef {j => w} {i => v}.
+
+Definition Precs {A T} R (m : ExchSig A R) : Prec T A :=
+  fun s ρs => exists ρ, ρs = eq ρ /\ (
+    CCleared s ρ \/
+    (exists i v, COffered i v s ρ) \/
+    (exists i j v w, CAccepted i j v w s ρ)).
+
+Definition Posts {A T} R (m : ExchSig A R) : Post T A R :=
+  fun _ _ _ => Precs R m.
+
+Definition Guar {T A} (i : Name T) : Relt T A :=
+  fun s ρs t σs => forall ρ, ρs = eq ρ -> exists σ, σs = eq σ /\ (
+    ( (* offer *)
+      CCleared s ρ /\
+      exists v, COffered i v t σ
+    ) \/
+    ( (* revoke *)
+      exists v,
+        COffered i v s ρ /\
+        CCleared t σ
+    ) \/
+    ( (* finish *)
+      exists j v w,
+        CAccepted j i w v s ρ /\
+        CCleared t σ
+    ) \/
+    ( (* accept *)
+      exists j w,
+        COffered j w s ρ /\
+        exists v,
+          CAccepted j i w v t σ
+    )
+  ).
+
+Definition ManyInvokeReturn {T A} i : Relt T A :=
+  RTC (fun s ρs t σs =>
+    exists j, j <> i /\
+      (InvokeAny (exchImpl A) j s ρs t σs \/
+       ReturnAny (exchImpl A) j s ρs t σs)).
+
+Definition Rely {T A} (i : Name T) : Relt T A :=
+  RTC (fun s ρs t σs =>
+    exists j, i <> j /\ (
+      Guar j s ρs t σs \/
+      InvokeAny (exchImpl A) j s ρs t σs \/
+      ReturnAny (exchImpl A) j s ρs t σs)).
+
+(* Tactics *)
+
+Ltac ddestruct H := dependent destruction H.
+
+Ltac elim_disj :=
+repeat match goal with
+| [ H : ?P \/ ?Q |- _] => destruct H
+end.
+
+Ltac decide_prop P :=
+  let H := fresh in
+  assert (H : P \/ ~P) by apply excluded_middle;
+  destruct H.
+
+Ltac set_ext x := extensionality x; apply propositional_extensionality.
+
+(* Helper lemmas *)
+
+Lemma TInvoke_pres_state {T A R} :
+  forall (m : F A R) i s ρ t σ,
+  TInvoke (VE:= VE T A) (VF:= VF T A) (exchImpl A) i R m s (eq ρ) t (eq σ) ->
+  PState ρ = PState σ /\
+  snd s = snd t.
+unfold TInvoke. intros. destruct_all.
+assert (σ = invPoss i ρ m).
+{
+  rewrite H2. exists ρ.
+  cbn. rewrite eqb_id.
+  repeat split; (easy || apply differ_pointwise_trivial).
+}
+subst. easy.
+Qed.
+
+Lemma TReturn_pres_state {T A R} :
+  forall (m : F A R) v i s ρ t σ,
+  TReturn (VE:= VE T A) (VF:= VF T A) (exchImpl A) i m v s (eq ρ) t (eq σ) ->
+  PState ρ = PState σ /\
+  snd s = snd t.
+unfold TReturn. intros. destruct_all.
+assert (σ = retPoss i ρ).
+{
+  rewrite H2. exists ρ.
+  specialize (H ρ eq_refl). destruct_all.
+  unfold mapRetPoss. cbn. rewrite eqb_id.
+  repeat split; (easy || apply differ_pointwise_trivial).
+}
+subst. easy.
+Qed.
+
+Lemma Invoke_pres_single {T A R} :
+  forall (m : F A R) i s ρ t σs,
+  TInvoke (VE:= VE T A) (VF:= VF T A) (exchImpl A) i R m s (eq ρ) t σs ->
+  exists σ, σs = eq σ.
+intros.
+unfold TInvoke in H. psimpl.
+exists (invPoss i ρ m).
+set_ext σ. split; intros; destruct_all; subst.
+{
+  unfold TIdle in H. destruct_all.
+  specialize (H2 x eq_refl). destruct_all.
+  destruct x, σ. unfold invPoss. cbn in *.
+  f_equal; try easy.
+  extensionality j. dec_eq_nats i j.
+  rewrite eqb_id. easy.
+  rewrite eqb_nid, H6; easy.
+  extensionality j. dec_eq_nats i j.
+  rewrite eqb_id. easy.
+  rewrite eqb_nid, H7; easy.
+}
+{
+  cbn. rewrite eqb_id. exists ρ.
+  repeat split; (easy || apply differ_pointwise_trivial).
+}
+Qed.
+
+Lemma Return_pres_single {T A R} :
+  forall (m : F A R) v i s ρ t σs,
+  TReturn (VE:= VE T A) (VF:= VF T A) (exchImpl A) i m v s (eq ρ) t σs ->
+  exists σ, σs = eq σ.
+intros.
+unfold TReturn, mapRetPoss in H. psimpl.
+exists (retPoss i ρ).
+set_ext σ. split; intros; destruct_all; subst.
+{
+  unfold retPoss. destruct x, σ. cbn in *.
+  f_equal. easy.
+  extensionality j. dec_eq_nats i j.
+  rewrite eqb_id. easy.
+  rewrite eqb_nid, H9; easy.
+  extensionality j. dec_eq_nats i j.
+  rewrite eqb_id. easy.
+  rewrite eqb_nid, H10; easy.
+}
+{
+  cbn. rewrite eqb_id. exists ρ.
+  specialize (H ρ eq_refl).
+  repeat split; (easy || apply differ_pointwise_trivial).
+}
+Qed.
+
+Lemma Rely_pres_single {T A} :
+  forall i s ρ t σs,
+  Rely (T:=T) (A:=A) i s (eq ρ) t σs ->
+  exists σ, σs = eq σ.
+Admitted.
+
+Lemma Rely_pres_self {T A} :
+  forall i s ρ t σ,
+  Rely (T:=T) (A:=A) i s (eq ρ) t (eq σ) ->
+  PCalls ρ i = PCalls σ i /\
+  PRets ρ i = PRets σ i.
+Admitted.
+
+Lemma eq_inj {A} :
+  forall x y : A, eq x = eq y -> x = y.
+intros.
+assert (forall z, eq x z = eq z y).
+{
+  intros. apply propositional_extensionality.
+  split; intros.
+  rewrite H in H0. easy.
+  rewrite H. easy.
+}
+specialize (H0 x).
+rewrite <- H0. easy.
+Qed.
+
+Lemma CAS_atomic {T A} :
+  forall i s ρ t σ a p,
+  Rely (T:=T) (A:=A) i s (eq ρ) t (eq σ) ->
+  snd s = CASDef a (Some p) ->
+  snd s = snd t /\
+  PState ρ = PState σ.
+intros.
+dependent induction H.
+apply eq_inj in x. subst. easy.
+destruct_all.
+Admitted.
+
+(* Subsidiary proofs *)
+
+Lemma Precs_stable {T A} :
+  forall (i : Name T) R (m : F A R),
+  Stable (Rely i) (Precs R m).
+unfold Stable, stablePrec, sub, subPrec.
+intros. psimpl. induction H0. easy.
+destruct_all. clear H1.
+apply IHRTC. clear IHRTC.
+elim_disj.
+2:{
+  unfold InvokeAny, TInvoke, TIdle in *. psimpl.
+  unfold Precs in *. psimpl.
+  exists (invPoss x x2 x1). split.
+  {
+    set_ext σ. split; intros; psimpl.
+    {
+      unfold invPoss. destruct x3, σ. cbn in *.
+      f_equal. easy.
+      extensionality j. dec_eq_nats x j.
+      rewrite eqb_id. easy.
+      rewrite eqb_nid, H9; easy.
+      extensionality j. dec_eq_nats x j.
+      rewrite eqb_id. easy.
+      rewrite eqb_nid, H10; easy.
+    }
+    {
+      exists x2. cbn. rewrite eqb_id.
+      repeat split; (easy || apply differ_pointwise_trivial).
+    }
+  }
+  {
+    unfold CCleared, COffered, CAccepted in *.
+    cbn in *. repeat rewrite <- H3. easy.
+  }
+}
+2:{
+  unfold ReturnAny, TReturn in *. psimpl.
+  unfold Precs in *. psimpl.
+  exists (retPoss x x3). split.
+  {
+    set_ext σ. split; intros; unfold mapRetPoss in *; psimpl.
+    {
+      unfold retPoss. destruct x4, σ. cbn in *.
+      f_equal. easy.
+      extensionality j. dec_eq_nats x j.
+      rewrite eqb_id. easy.
+      rewrite eqb_nid, H11; easy.
+      extensionality j. dec_eq_nats x j.
+      rewrite eqb_id. easy.
+      rewrite eqb_nid, H12; easy.
+    }
+    {
+      exists x3. cbn. rewrite eqb_id.
+      specialize (H1 x3 eq_refl). destruct_all.
+      repeat split; (easy || apply differ_pointwise_trivial).
+    }
+  }
+  {
+    unfold CCleared, COffered, CAccepted in *.
+    cbn in *. repeat rewrite <- H3. easy.
+  }
+}
+{
+  unfold Precs, Guar in *. psimpl.
+  specialize (H1 x0 eq_refl). psimpl.
+  exists x1. split. easy.
+  destruct H1; destruct_all.
+  2: destruct H; destruct_all.
+  3: destruct H; destruct_all.
+  right. left. exists x, x2. easy.
+  left. easy.
+  left. easy.
+  {
+    right. right.
+    unfold CCleared, CAccepted, COffered in *. destruct_all.
+    elim_disj; destruct_all.
+    { rewrite H2 in H. discriminate. }
+    2:{ rewrite H6 in H. discriminate. }
+    {
+      rewrite H2 in H. clear H2. ddestruct H.
+      rewrite H6 in H5. clear H6. ddestruct H5.
+      apply insert_cong in x. psimpl. clear H2.
+      ddestruct H. rewrite H3, H4. clear H3 H4.
+      exists x2, x4, x3, x6. easy.
+    }
+  }
+}
+Qed.
+
+Definition PossSetSteps {T F} {VF : Spec T F} (ρs σs : PossSet VF) :=
+  forall σ, σs σ ->
+    exists ρ, ρs ρ /\
+      PossSteps ρ σ.
+
+Lemma lemCAS {T A} {i : Name T} :
+  forall e n (P : Relt T A),
+  forall (PS PF : Poss (VF T A) -> Poss (VF T A) -> Prop),
+  (forall s ρ σ,
+    ReltToPrec P s (eq ρ) ->
+    snd s = CASDef e None ->
+    PState ρ = PState σ ->
+    PCalls ρ i = PCalls σ i ->
+    PRets ρ i = PRets σ i ->
+    exists τ,
+      PossSteps σ τ /\
+      PS σ τ) ->
+  (forall s ρ σ,
+    ReltToPrec P s (eq ρ) ->
+    (exists a,
+      a <> e /\
+      snd s = CASDef a None) ->
+    PState ρ = PState σ ->
+    PCalls ρ i = PCalls σ i ->
+    PRets ρ i = PRets σ i ->
+    exists τ,
+      PossSteps σ τ /\
+      PF σ τ) ->
+  (forall s ρs,
+    ReltToPrec P s ρs ->
+    exists ρ,
+      ρs = eq ρ) ->
+  VerifyProg i (Rely i) (Guar i)
+    P
+    (call (CAS e n))
+    (fun v s ρs r τs =>
+      exists ρ, ρs = eq ρ /\
+      exists τ, τs = eq τ /\
+      exists t σ,
+        PState ρ = PState σ /\
+        PCalls ρ i = PCalls σ i /\
+        PRets ρ i = PRets σ i /\
+        ((v = true /\
+          snd s = CASDef e None /\
+          snd t = CASDef n None /\
+          PS σ τ /\
+          Rely i t (eq σ) r (eq τ)) \/
+        (v = false /\
+          (exists a,
+            a <> e /\
+            snd s = CASDef a None) /\
+          snd t = CASDef n None /\
+          PF σ τ /\
+          Rely i t (eq σ) r (eq τ)))).
+intros.
+eapply weakenPost.
+{
+  eapply (lemCall
+    (Q:=fun (s : InterState (F A) (VE T A)) ρs t σs =>
+      (exists ρ, ρs = eq ρ /\ exists σ, σs = eq σ /\
+        PState ρ = PState σ /\
+        PCalls ρ i = PCalls σ i /\
+        PRets ρ i = PRets σ i) /\
+      (exists a,
+        snd s = CASDef a None /\
+        snd t = CASDef a (Some (MkCASPend i (CAS e n)))))
+    (S:=fun v t σs r τs =>
+      exists σ, σs = eq σ /\
+      exists τ, τs = eq τ /\
+      (v = true /\
+        PS σ τ /\
+        Rely i t (eq σ) r (eq τ)) \/
+      (v = false /\
+        PF σ τ /\
+        Rely i t (eq σ) r (eq τ)))).
+  {
+    admit.
+  }
+  {
+    admit.
+  }
+  {
+    unfold Commit. intros. psimpl.
+    
+  }
+}
+
+Lemma exch_correct {T A} {i : Name T} :
+  forall v,
+  VerifyProg i (Rely i) (Guar i)
+    (prComp (Precs (option A) (Exch v)) (TInvoke (exchImpl A) i _ (Exch v)) ->> Rely i)
+    (exch v)
+    (fun v' => Posts _ (Exch v) v' ->> PrecToRelt (Returned i (Exch v))).
+unfold exch. intros.
+eapply lemBind.
+{
+  
+}
+
+
+(* Result *)
+
+Theorem ticketLockCorrect T A :
+  VerifyImpl (VE T A) (VF T A) Rely Guar (fun _ => Precs) (exchImpl A) (fun _ => Posts).
+constructor.
+{
+  constructor.
+}
+{
+  unfold Rely, sub, subRelt. intros. psimpl.
+  apply rtcTrans. psplit. exact H. easy.
+}
+{
+  unfold Rely, sub, subRelt. intros.
+  econstructor. 2: constructor.
+  exists i. split. easy. left. easy.
+}
+{
+  unfold Rely, sub, subRelt. intros.
+  econstructor. 2: constructor.
+  exists i. split. easy. right. left. easy.
+}
+{
+  unfold Rely, sub, subRelt. intros.
+  econstructor. 2: constructor.
+  exists i. split. easy. right. right. easy.
+}
+{
+  exists initPoss. split. easy. left. easy.
+}
+{
+  apply Precs_stable.
+}
+{
+  unfold Stable, stableRelt, Posts, sub, subRelt. intros. psimpl.
+  eapply Precs_stable. psplit.
+  exact H. exact H0.
+}
+{
+  unfold sub, subPrec. intros. psimpl.
+  unfold Posts, Precs, CCleared, COffered, CAccepted in *.
+  psimpl.
+  assert (exists τ, ρ = eq τ).
+  eapply Return_pres_single. exact H0. psimpl.
+  exists x0. split. easy.
+  apply TReturn_pres_state in H0. destruct_all.
+  rewrite <- H. clear H4.
+  elim_disj.
+  {
+    left.
+    rewrite <- H0 at 1. easy.
+  }
+  {
+    right. left. destruct_all.
+    rewrite H0 in H2 at 1.
+    exists x4, x5. easy.
+  }
+  {
+    right. right. destruct_all.
+    rewrite H0 in H3 at 1.
+    exists x4, x5, x6, x7. easy.
+  }
+}
+{
+  intros. destruct m. cbn.
+  apply exch_correct.
+}
+Qed.
