Examples/ExchangerSpec.v
@@ -1,0 +1,48 @@
+From LHL.Core Require Import
+  Program
+  Specs.
+
+From LHL.Util Require Import
+  Util.
+
+Variant ExchSig {A} : ESig :=
+| Exch (v : A) : ExchSig (option A).
+Arguments ExchSig : clear implicits.
+
+Variant ExchState {T A} :=
+| ExchDef (p d : set (Name T * A)).
+Arguments ExchState : clear implicits.
+
+Notation "{}" := emp.
+Notation "{ i => x }" := (insert (i, x) emp).
+Notation "{ i => x , j => y }" := (insert (i, x) (insert (j, y) emp)).
+
+Variant ExchStep {T A} : ExchState T A -> ThreadEvent T (ExchSig A) -> ExchState T A -> Prop :=
+| ExchCall1 i x : ExchStep
+    (ExchDef {} {})
+    (i, CallEv (Exch x))
+    (ExchDef {i => x} {})
+| ExchCall2 i x j y : i <> j -> ExchStep
+    (ExchDef {i => x} {})
+    (j, CallEv (Exch y))
+    (ExchDef {i => x, j => y} {})
+| ExchRet1 i x j y : i <> j -> ExchStep
+    (ExchDef {i => x, j => y} {})
+    (i, RetEv (Exch x) (Some y))
+    (ExchDef {i => x} {j => y})
+| ExchRet2 i x j y : i <> j -> ExchStep
+    (ExchDef {i => x} {j => y})
+    (j, RetEv (Exch y) (Some x))
+    (ExchDef {} {})
+| ExchFail i x : ExchStep
+    (ExchDef {i => x} {})
+    (i, RetEv (Exch x) None)
+    (ExchDef {} {}).
+
+Program Definition exchSpec {T A} : Spec T (ExchSig A) := {|
+  State := ExchState T A;
+  Step := ExchStep;
+  Init := ExchDef {} {}
+|}.
+
+Admit Obligations.
