Examples/MRSWCellSpec.v
@@ -7,27 +7,27 @@ Variant CellSig {A} : ESig :=
 | Read : CellSig A.
 Arguments CellSig : clear implicits.
 
-Record CellPend {A} := MkCellPend {
-  CellThread : ThreadName;
+Record CellPend {T A} := MkCellPend {
+  CellThread : Name T;
   CellRetTy : Type;
   CellName : CellSig A CellRetTy
 }.
 Arguments CellPend : clear implicits.
-Arguments MkCellPend {A}.
+Arguments MkCellPend {T A}.
 
-Variant CellState {A} :=
+Variant CellState {T A} :=
 | CellUB (* todo: make sequentially consistent *)
-| CellDef (v : option A) (m : option (CellPend A)).
+| CellDef (v : option A) (m : option (CellPend T A)).
 Arguments CellState : clear implicits.
 
-Definition CellUndef {A} := @CellDef A None None.
-Definition CellIdle {A} (v : option A) := CellDef v None.
-Definition CellWriteRan {A} i v (v' : A) :=
-  CellDef v (Some (MkCellPend i _ (Write v'))).
-Definition CellReadRan {A} i (v : A) :=
-  CellDef (Some v) (Some (MkCellPend i _ Read)).
+Definition CellUndef {T A} := @CellDef T A None None.
+Definition CellIdle {T A} (v : option A) := CellDef (T:=T) v None.
+Definition CellWriteRan {T A} i v (v' : A) :=
+  CellDef (T:=T) v (Some (MkCellPend i _ (Write v'))).
+Definition CellReadRan {T A} i (v : A) :=
+  CellDef (T:=T) (Some v) (Some (MkCellPend i _ Read)).
 
-Variant CellStep {A} : CellState A -> ThreadEvent (CellSig A) -> CellState A -> Prop :=
+Variant CellStep {T A} : CellState T A -> ThreadEvent T (CellSig A) -> CellState T A -> Prop :=
 | CellCallWrite i v v' :
     CellStep (CellIdle v) (i, CallEv (Write v')) (CellWriteRan i v v')
 | CellRetWrite i v v' :
@@ -39,16 +39,13 @@ Variant CellStep {A} : CellState A -> ThreadEvent (CellSig A) -> CellState A -> 
 | CellDoubleWrite i j v v' v'' :
     i <> j ->
     CellStep (CellWriteRan i v v') (j, CallEv (Write v'')) CellUB
-| CellDoubleRead i j v :
-    i <> j ->
-    CellStep (CellReadRan i v) (j, CallEv Read) CellUB
 | CellReadUndef i :
     CellStep (CellIdle None) (i, CallEv Read) CellUB
 | CellStepUB e :
     CellStep CellUB e CellUB.
 
-Program Definition cellSpec A : Spec (CellSig A) := {|
-  State := CellState A;
+Program Definition cellSpec {T A} : Spec T (CellSig A) := {|
+  State := CellState T A;
   Step := CellStep;
   Init := CellUndef
 |}.
