Examples/NameSpec.v
@@ -1,0 +1,35 @@
+From LHL.Core Require Import
+  Program
+  Specs
+  Logic.
+
+From LHL.Util Require Import
+  Tactics
+  TransUtil
+  Util.
+
+Variant NameSig {T} : ESig :=
+| Self : NameSig (Name T).
+Arguments NameSig : clear implicits.
+
+Definition NameState T := ActiveMap T (NameSig T).
+
+Variant NameStep {T} : NameState T -> ThreadEvent T (NameSig T) -> NameState T -> Prop :=
+| CallSelf i m m' :
+    m i = None ->
+    m' i = Some (existT _ _ Self) ->
+    differ_pointwise m m' i ->
+    NameStep m (i, CallEv Self) m'
+| RetSelf i m m' :
+    m i = Some (existT _ _ Self) ->
+    m' i = None ->
+    differ_pointwise m m' i ->
+    NameStep m (i, RetEv Self i) m'.
+
+Program Definition nameSpec {T} : Spec T (NameSig T) := {|
+  State := NameState T;
+  Step := NameStep;
+  Init _ := None
+|}.
+
+Admit Obligations.
