Examples/WkSpec.v
@@ -1,0 +1,38 @@
+From LHL.Core Require Import
+  Specs
+  Traces
+  Program.
+
+From LHL.Util Require Import
+  TransUtil
+  Util.
+
+Variant WkState {T E A} :=
+| UB (m : ActiveMap T E)
+| Def (v : A).
+Arguments WkState : clear implicits.
+
+Variant WkStep {T E} {V : Spec T E} : WkState T E V.(State) -> ThreadEvent T E -> WkState T E V.(State) -> Prop :=
+| DefStep s e t :
+    V.(Step) s e t ->
+    WkStep (Def s) e (Def t)
+| TrigUB s e :
+    (forall t, ~V.(Step) s e t) ->
+    WkStep (Def s) e (UB (fun _ => None))
+| CallUB a a' i A (m : E A) :
+    a i = None ->
+    a' i = Some (existT _ _ m) ->
+    WkStep (UB a) (i, CallEv m) (UB a')
+| RetUB a a' i A (m : E A) v :
+    a i = Some (existT _ _ m) ->
+    a' i = None ->
+    WkStep (UB a) (i, RetEv m v) (UB a').
+Arguments WkStep {T E} V.
+
+Program Definition wkSpec {T E} (V : Spec T E) : Spec T E := {|
+  State := WkState T E V.(State);
+  Step := WkStep V;
+  Init := Def V.(Init)
+|}.
+
+Next Obligation.
